<?xml version="1.0" encoding="UTF-8"?>
<rdf:RDF
   xmlns:dc="http://purl.org/dc/elements/1.1/"
   xmlns:dct="http://purl.org/dc/terms/"
   xmlns:owl="http://www.w3.org/2002/07/owl#"
   xmlns:rdf="http://www.w3.org/1999/02/22-rdf-syntax-ns#"
   xmlns:rdfs="http://www.w3.org/2000/01/rdf-schema#"
   xmlns:sdo="https://schema.org/"
   xmlns:skos="http://www.w3.org/2004/02/skos/core#"
>
  <rdf:Description rdf:about="http://www.w3.org/ns/dx/prof/hasToken">
    <rdfs:domain rdf:resource="http://www.w3.org/ns/dx/prof/Profile"/>
    <skos:definition xml:lang="en">The preferred identifier for the Profile, for use in circumstances where its URI cannot be used</skos:definition>
    <rdfs:range rdf:resource="http://www.w3.org/2001/XMLSchema#token"/>
    <skos:usageNote xml:lang="en">A simple lexical form of identifier that may be accepted in some circumstances, such as API arguments to reference this profile. This is the 'preferred term', since alternative identifiers may be declared and used by any implementation</skos:usageNote>
    <rdf:type rdf:resource="http://www.w3.org/2002/07/owl#DatatypeProperty"/>
    <rdfs:label>has token</rdfs:label>
  </rdf:Description>
  <rdf:Description rdf:about="http://www.w3.org/ns/dx/prof/isTransitiveProfileOf">
    <skos:usageNote xml:lang="en">This is a convenience property that may be used to access all specifications (including other profiles) that could provide useful information and related resources for the Profile (for example, for better identifying conformance requirements). This avoids forcing clients to traverse a profile hierarchy to find all relevant resources. If this property is used, then all such relationships should be present so a client can safely avoid hierarchy traversal</skos:usageNote>
    <skos:definition xml:lang="en">The transitive closure of the :isProfileOf property. Relates a profile to another specification that it is a profile of, possibly via a chain of intermediate profiles that are in :isProfileOf relationships</skos:definition>
    <rdfs:domain rdf:resource="http://www.w3.org/ns/dx/prof/Profile"/>
    <rdfs:range rdf:resource="http://purl.org/dc/terms/Standard"/>
    <rdf:type rdf:resource="http://www.w3.org/2002/07/owl#ObjectProperty"/>
    <rdfs:label>is transitive profile of</rdfs:label>
  </rdf:Description>
  <rdf:Description rdf:about="http://www.w3.org/ns/dx/prof/isProfileOf">
    <rdfs:range rdf:resource="http://purl.org/dc/terms/Standard"/>
    <rdf:type rdf:resource="http://www.w3.org/2002/07/owl#ObjectProperty"/>
    <skos:usageNote xml:lang="en">A Profile may define constraints on the usage of one or more specifications. All constraints of these specifications are inherited, in the sense that an object conforming to a profile conforms to all the constraints specified the targets of :isProfileOf relations. This property is optional, allowing any specification to be declared at the root of a profile hierarchy using the Profile class</skos:usageNote>
    <rdfs:subPropertyOf rdf:resource="http://www.w3.org/ns/dx/prof/isTransitiveProfileOf"/>
    <skos:definition xml:lang="en">A specification for which this Profile defines constraints, extensions, or which it uses in combination with other specifications, or provides guidance or explanation about its usage</skos:definition>
    <rdfs:domain rdf:resource="http://www.w3.org/ns/dx/prof/Profile"/>
    <rdfs:label>is profile of</rdfs:label>
  </rdf:Description>
  <rdf:Description rdf:about="http://www.w3.org/ns/dx/prof">
    <rdfs:comment xml:lang="en">This vocabulary is for describing relationships between standards/specifications, profiles of them and supporting artifacts such as validating resources.

This model starts with [http://dublincore.org/2012/06/14/dcterms#Standard](dct:Standard) entities which can either be Base Specifications (a standard not profiling any other Standard) or Profiles (Standards which do profile others). Base Specifications or Profiles can have Resource Descriptors associated with them that defines implementing rules for the it. Resource Descriptors must indicate the role they play (to guide, to validate etc.) and the formalism they adhere to (dct:format) to allow for content negotiation. A vocabulary of Resource Roles are provided alongside this vocabulary but that list is extensible.</rdfs:comment>
    <dct:contributor rdf:resource="http://orcid.org/0000-0002-8742-7730"/>
    <dc:contributor>Makx Dekkers</dc:contributor>
    <dct:modified rdf:datatype="http://www.w3.org/2001/XMLSchema#date">2019-10-25</dct:modified>
    <owl:versionIRI rdf:resource="http://www.w3.org/ns/dx/prof/1.0"/>
    <dc:contributor>Alejandra Gonzalez-Beltran</dc:contributor>
    <dct:creator rdf:nodeID="ub462bL15C45"/>
    <dc:contributor>Antoine Isaac</dc:contributor>
    <dc:contributor>Simon Cox</dc:contributor>
    <dct:created rdf:datatype="http://www.w3.org/2001/XMLSchema#date">2018-02-16</dct:created>
    <rdfs:label>Profiles Vocabulary</rdfs:label>
    <dct:creator rdf:nodeID="ub462bL24C33"/>
    <owl:versionInfo>1.0</owl:versionInfo>
    <rdf:type rdf:resource="http://www.w3.org/2002/07/owl#Ontology"/>
  </rdf:Description>
  <rdf:Description rdf:about="http://purl.org/dc/terms/conformsTo">
    <skos:definition xml:lang="en">An established standard to which the described resource conforms</skos:definition>
    <rdfs:isDefinedBy rdf:resource="http://purl.org/dc/terms/"/>
    <rdfs:range rdf:resource="http://purl.org/dc/terms/Standard"/>
    <rdfs:subPropertyOf rdf:resource="http://purl.org/dc/elements/1.1/relation"/>
    <rdfs:subPropertyOf rdf:resource="http://purl.org/dc/terms/relation"/>
    <owl:propertyChainAxiom rdf:nodeID="f2b608390d12a458a99f33842150f70b2b1"/>
    <skos:scopeNote>This property is to be used to show conformance of a data resource to a specification (dct:Standard) or a profile (:Profile).

The property chain axiom declared for this property means that if the thing conformed to is a profile of something else (indicated by :isProfileOf), then the conforming data resource will be inferred to be conformant to that other thing too.

PROF does not specify the nature of conformance: communities using specifications and profiles are free to define appropriate conformance for their purposes.</skos:scopeNote>
    <rdfs:label>conforms to</rdfs:label>
    <rdf:type rdf:resource="http://www.w3.org/2002/07/owl#AnnotationProperty"/>
  </rdf:Description>
  <rdf:Description rdf:about="http://www.w3.org/ns/dx/prof/ResourceRole">
    <skos:definition xml:lang="en">A role that an profile resource, described by a Resource Descriptor, plays</skos:definition>
    <rdfs:label>Resource Role</rdfs:label>
    <rdf:type rdf:resource="http://www.w3.org/2002/07/owl#Class"/>
    <rdfs:subClassOf rdf:resource="http://www.w3.org/2004/02/skos/core#Concept"/>
    <skos:usageNote xml:lang="en">Specific terms must come from a vocabulary</skos:usageNote>
  </rdf:Description>
  <rdf:Description rdf:nodeID="ub462bL24C33">
    <sdo:affiliation rdf:nodeID="ub462bL28C53"/>
    <sdo:affiliation rdf:nodeID="ub462bL32C37"/>
    <sdo:name>Rob Atkinson</sdo:name>
    <sdo:identifier rdf:resource="http://orcid.org/0000-0002-7878-2693"/>
    <sdo:email rdf:resource="http://www.w3.org/ns/dx/rob@metalinkage.com.au"/>
  </rdf:Description>
  <rdf:Description rdf:nodeID="ub462bL15C45">
    <sdo:name>Nicholas J. Car</sdo:name>
    <sdo:affiliation rdf:nodeID="ub462bL19C53"/>
    <sdo:identifier rdf:resource="http://orcid.org/0000-0002-8742-7730"/>
    <sdo:email rdf:resource="http://www.w3.org/ns/dx/nicholas.car@surroundaustralia.com"/>
  </rdf:Description>
  <rdf:Description rdf:nodeID="ub462bL32C37">
    <sdo:name>Metalinkage</sdo:name>
  </rdf:Description>
  <rdf:Description rdf:nodeID="f2b608390d12a458a99f33842150f70b2b1">
    <rdf:rest rdf:nodeID="f2b608390d12a458a99f33842150f70b2b2"/>
    <rdf:first rdf:resource="http://www.w3.org/ns/dx/prof/isProfileOf"/>
  </rdf:Description>
  <rdf:Description rdf:about="http://www.w3.org/ns/dx/prof/hasArtifact">
    <rdfs:domain rdf:resource="http://www.w3.org/ns/dx/prof/ResourceDescriptor"/>
    <skos:definition xml:lang="en">The URL of a downloadable file with particulars such as its format and role indicated by the Resource Descriptor</skos:definition>
    <rdf:type rdf:resource="http://www.w3.org/2002/07/owl#ObjectProperty"/>
    <rdfs:label>has artifact</rdfs:label>
    <skos:usageNote xml:lang="en">A property to link from a Resource Descriptor to an actual information resource (rdfs:Resource; an individual) that implements it</skos:usageNote>
  </rdf:Description>
  <rdf:Description rdf:nodeID="ub462bL28C53">
    <sdo:name>Open Geospatial Consortium</sdo:name>
    <sdo:url rdf:resource="https://www.opengeospatial.org/"/>
  </rdf:Description>
  <rdf:Description rdf:about="http://www.w3.org/ns/dx/prof/hasResource">
    <rdf:type rdf:resource="http://www.w3.org/2002/07/owl#ObjectProperty"/>
    <rdfs:label xml:lang="en">has resource</rdfs:label>
    <skos:definition xml:lang="en">A resource which describes the nature of an artifact and the role it plays in relation to the Profile</skos:definition>
    <skos:usageNote xml:lang="en">This property is analogous to dcat:distribution however the domain is not necessarily dcat:Dataset. dcat:Dataset and :Profile are not disjoint, so it is up to implementations to decide if these are equivalent properties</skos:usageNote>
    <rdfs:range rdf:resource="http://www.w3.org/ns/dx/prof/ResourceDescriptor"/>
  </rdf:Description>
  <rdf:Description rdf:about="http://www.w3.org/ns/dx/prof/isInheritedFrom">
    <rdfs:domain rdf:resource="http://www.w3.org/ns/dx/prof/ResourceDescriptor"/>
    <rdf:type rdf:resource="http://www.w3.org/2002/07/owl#ObjectProperty"/>
    <rdfs:range rdf:resource="http://www.w3.org/ns/dx/prof/Profile"/>
    <skos:usageNote xml:lang="en">This property is created for the convenience of clients. When profile describers wish to allow clients to discover all resources relevant to a Profile without having to navigating an inheritance hierarchy of :profileOf relations, this predicate may be used to directly associate inherited Profile Descriptors with the Profile. If this property is present, it should be used consistently and all relevant resources a client may need to utilise the profile should be present and described using this predicate</skos:usageNote>
    <skos:definition xml:lang="en">A base specification, a Resource Descriptor from which is to be considered a Resource Descriptor for this Profile also</skos:definition>
    <rdfs:label>is inherited from</rdfs:label>
  </rdf:Description>
  <rdf:Description rdf:about="http://purl.org/dc/terms/format">
    <rdfs:subPropertyOf rdf:resource="http://purl.org/dc/elements/1.1/format"/>
    <rdf:type rdf:resource="http://www.w3.org/2002/07/owl#AnnotationProperty"/>
    <rdfs:range rdf:resource="http://purl.org/dc/terms/MediaTypeOrExtent"/>
  </rdf:Description>
  <rdf:Description rdf:nodeID="ub462bL19C53">
    <sdo:name>SURROUND Australia Pty Ltd</sdo:name>
    <sdo:url rdf:resource="https://surroundaustralia.com"/>
  </rdf:Description>
  <rdf:Description rdf:about="http://www.w3.org/ns/dx/prof/hasRole">
    <rdfs:domain rdf:resource="http://www.w3.org/ns/dx/prof/ResourceDescriptor"/>
    <rdfs:label>has role</rdfs:label>
    <skos:definition xml:lang="en">The function of an artifact described by a Resource Descriptor, such as specification, guidance etc.</skos:definition>
    <rdf:type rdf:resource="http://www.w3.org/2002/07/owl#ObjectProperty"/>
    <rdfs:range rdf:resource="http://www.w3.org/2004/02/skos/core#Concept"/>
    <skos:usageNote xml:lang="en">A set of common roles are defined by the Profiles Vocabulary. These are not exhaustive or disjoint, and may be extended for situations where finer grained description of purpose is necessary. A resource may perform multiple roles</skos:usageNote>
  </rdf:Description>
  <rdf:Description rdf:about="http://www.w3.org/ns/dx/prof/ResourceDescriptor">
    <skos:definition xml:lang="en">A description of a resource that defines an aspect - a particular part, feature or role - of a Profile</skos:definition>
    <rdf:type rdf:resource="http://www.w3.org/2002/07/owl#Class"/>
    <skos:usageNote xml:lang="en">Can be use to indicate the formalism (via dct:format) and any adherence to a dct:Standard (via dct:conformsTo) to allow for machine mediation as well as its purpose via relation to a ResourceRole (via hasRole)</skos:usageNote>
    <rdfs:label xml:lang="en">Resource Descriptor</rdfs:label>
  </rdf:Description>
  <rdf:Description rdf:about="http://www.w3.org/ns/dx/prof/Profile">
    <rdfs:label>Profile</rdfs:label>
    <rdf:type rdf:resource="http://www.w3.org/2002/07/owl#Class"/>
    <skos:definition xml:lang="en">A specification that constrains, extends, combines, or provides guidance or explanation about the usage of other specifications.

This definition includes what are often called "application profiles", "metadata application profiles", or "metadata profiles".</skos:definition>
    <rdfs:subClassOf rdf:resource="http://purl.org/dc/terms/Standard"/>
    <dct:source rdf:resource="https://www.w3.org/2017/dxwg/wiki/ProfileContext"/>
  </rdf:Description>
  <rdf:Description rdf:nodeID="f2b608390d12a458a99f33842150f70b2b2">
    <rdf:first rdf:resource="http://purl.org/dc/terms/conformsTo"/>
    <rdf:rest rdf:resource="http://www.w3.org/1999/02/22-rdf-syntax-ns#nil"/>
  </rdf:Description>
</rdf:RDF>
